coq/LLVMGen/Correctness_GenIR.v
@@ -76,6 +76,23 @@ Axiom int_eq_inv: forall a b, Int64.intval a ≡ Int64.intval b -> a ≡ b.
     Opaque incVoid.
   Qed.
 
+  (* TODO: move this? *)
+  Lemma incLocal_id_neq :
+    forall s1 s2 s3 s4 id1 id2,
+      incLocal s1 ≡ inr (s2, id1) ->
+      incLocal s3 ≡ inr (s4, id2) ->
+      local_count s1 ≢ local_count s3 ->
+      id1 ≢ id2.
+  Proof.
+    intros s1 s2 s3 s4 id1 id2 GEN1 GEN2 COUNT.
+    eapply incLocalNamed_count_gen_injective.
+    symmetry. rewrite incLocal_unfold in *. eapply GEN1.
+    symmetry. rewrite incLocal_unfold in *. eapply GEN2.
+    solve_local_count_tac.
+    solve_not_ends_with.
+    solve_not_ends_with.
+  Qed.
+
   Lemma genNExpr_context :
     forall nexp s1 s2 e c,
       genNExpr nexp s1 ≡ inr (s2, (e,c)) ->
